src/tools/parallelcomposition/propertyScript.sml
@@ -1,0 +1,110 @@
+open HolKernel Parse boolLib bossLib;
+open sumTheory;
+open pred_setTheory;
+
+val _ = new_theory "propert";
+    
+(* Trace *)
+val _ = Parse.type_abbrev("trc", ``:'event list``);  
+
+val (trace_rules, trace_ind, trace_cases)
+= Hol_reln
+  `(((MTS = (MTrn,Ded)) ∧ (MTrn ({},{},st0) [] ({},{},st0))) ==> (trace MTS [])) ∧
+(((MTS = (MTrn,Ded)) ∧ (MTrn ({},{},st0) Evs Conf)) ==> (trace MTS Evs)) ∧
+(((MTS = (MTrn,Ded)) ∧ (MTrn ({},{},st0) Evs Conf) ∧ (Trn Conf Ev Conf') ∧ (MTS' = (MTrn',Ded')) ∧ (MTrn' ({},{},st0) (Ev::Evs) Conf')) ==> (trace MTS' (Ev::Evs)))
+`;
+
+
+(* Trace property NOT*)
+val tracePropertyNot_def =
+Define`
+tracePropertyNot (Phi:( 'event trc set)) = {t|(t ∉ Phi) ∧ (TL(t) ∈ Phi)}
+                                                           `;
+
+val _ = overload_on ("¬", ``tracePropertyNot``);
+
+(* Traces *)
+val traces_def =
+Define`
+traces MTS Phi = {t| (trace MTS t) ∧ (t ∈ (tracePropertyNot Phi))}
+`;
+
+
+(* Satisfy Trace property *)
+val satisfyTraceProperty_def =
+Define`
+satisfyTraceProperty MTS Phi = ((traces MTS Phi) ⊆ Phi)
+                                                           `;
+val _ = set_mapped_fixity { fixity = Infixl 90,
+                            term_name = "apply_satisfyTraceProperty",
+                            tok = "⊨" };
+
+val _ = overload_on ("apply_satisfyTraceProperty", ``satisfyTraceProperty``);    
+
+
+(* Trace refinement *)
+val traceRefinement_def =
+Define`
+      traceRefinement MTS1 MTS2 = (∀Phi. ((traces MTS1 Phi) ⊆ (traces MTS2 Phi)))
+                                                                                                                              `;
+val _ = set_mapped_fixity { fixity = Infixl 95,
+                            term_name = "apply_traceRefinement",
+                            tok = "⊑" };
+
+val _ = overload_on ("apply_traceRefinement", ``traceRefinement``);
+
+
+(* Inductive state simulation *)
+val (stateSimulation_rules, stateSimulation_ind, stateSimulation_cases) =
+Hol_reln`
+        ((((MTS1 = (MTrn1,Ded1)) ∧ (MTrn1 Conf1 Evs Conf1')) ⇒ (∃(Conf2':(('symb set) # ('pred set) # 'state)). (MTS2 = (MTrn2,Ded2)) ∧ (MTrn2 Conf2 Evs Conf2') ∧ (stateSimulation (MTS1,Conf1) (MTS2,Conf2)))) ==> (stateSimulation (MTS1,Conf1') (MTS2,Conf2'))) ∧
+((((MTS1 = (MTrn1,Ded1)) ∧ (MTrn1 ({},{},st01) Evs Conf1)) ⇒ (∃(Conf2:(('symb set) # ('pred set) # 'state)). (MTS2 = (MTrn2,Ded2)) ∧ (MTrn2 ({},{},st02) Evs Conf2) ∧ (stateSimulation (MTS1,({},{},st01)) (MTS2,({},{},st02))))) ==> (stateSimulation (MTS1,Conf1) (MTS2,Conf2))) 
+`;
+
+val _ = set_mapped_fixity { fixity = Infixl 95,
+                            term_name = "apply_stateSimulation",
+                            tok = "≼" };
+
+val _ = overload_on ("apply_stateSimulation", ``stateSimulation``);
+
+
+(* Simulation *)
+val (simulation_rules, simulation_ind, simulation_cases) =
+Hol_reln`
+          ((stateSimulation (MTS1,({},{},st01)) (MTS2,({},{},st02))) ==> (simulation MTS1 MTS2))  
+          `;
+    
+val _ = set_mapped_fixity { fixity = Infixl 95,
+                            term_name = "apply_simulation",
+                            tok = "≲" };
+
+val _ = overload_on ("apply_simulation", ``simulation``);
+
+
+ (*
+val sim_vs_ref_thm = store_thm(
+  "sim_vs_ref_thm", ``!(MTS1:((α -> bool) # (β -> bool) # γ ->
+                              δ list -> (α -> bool) # (β -> bool) # γ -> bool) # ε) (MTS2:((α -> bool) # (β -> bool) # γ ->
+                                                                                           δ list -> (α -> bool) # (β -> bool) # γ -> bool) # ε).
+                       (MTS1 ≲ MTS2) ==> (MTS1 ⊑ MTS2) ``
+  ,
+  
+  REPEAT GEN_TAC >>        
+  REWRITE_TAC [simulation_cases]>>
+  STRIP_TAC >>
+  REWRITE_TAC [traceRefinement_def,traces_def,trace_cases]>>
+  STRIP_TAC >>          
+  Cases_on `MTS1 = MTS2`  >| [
+      ALL_TAC
+      ,
+      ASM_SIMP_TAC (std_ss++pred_setSimps.PRED_SET_ss) []
+    ] >>
+  REWRITE_TAC [tracePropertyNot_def]>>
+  METIS_TAC [stateSimulation_rules, stateSimulation_ind, stateSimulation_cases]
+  );
+WIP on the proof-no cheat but METIS_TAC could not find proof *)
+  
+val _ = export_theory();
+
+(* DB.find_in "SET" (DB.find "SUM_MAP"); *)
+(* DB.find "SET_CASES_TAC"; *)
